chore: renaming

CollapsingTowers/TwoLevelPCP/OpenClose.lean
@@ -6,11 +6,11 @@ import CollapsingTowers.TwoLevelPCP.Syntax
 def subst (x : ℕ) (v : Expr) : Expr → Expr
   | .bvar i => .bvar i
   | .fvar y => if x = y then v else .fvar y
-  | .lam₁ e => .lam₁ (subst x v e)
+  | .lam e => .lam (subst x v e)
   | .lift e => .lift (subst x v e)
   | .app₁ f arg => .app₁ (subst x v f) (subst x v arg)
   | .app₂ f arg => .app₂ (subst x v f) (subst x v arg)
-  | .lit₁ n => .lit₁ n
+  | .lit n => .lit n
   | .binary₁ op l r => .binary₁ op (subst x v l) (subst x v r)
   | .binary₂ op l r => .binary₂ op (subst x v l) (subst x v r)
   | .run e => .run (subst x v e)
@@ -36,11 +36,11 @@ def subst (x : ℕ) (v : Expr) : Expr → Expr
 def opening (i : ℕ) (x : Expr) : Expr → Expr
   | .bvar j => if j = i then x else .bvar j
   | .fvar x => .fvar x
-  | .lam₁ e => .lam₁ (opening (i + 1) x e)
+  | .lam e => .lam (opening (i + 1) x e)
   | .lift e => .lift (opening i x e)
   | .app₁ f arg => .app₁ (opening i x f) (opening i x arg)
   | .app₂ f arg => .app₂ (opening i x f) (opening i x arg)
-  | .lit₁ n => .lit₁ n
+  | .lit n => .lit n
   | .binary₁ op l r => .binary₁ op (opening i x l) (opening i x r)
   | .binary₂ op l r => .binary₂ op (opening i x l) (opening i x r)
   | .run e => .run (opening i x e)
@@ -73,11 +73,11 @@ def open_subst (tgt : Expr) (within : Expr) :=
 def closing (i : ℕ) (x : ℕ) : Expr → Expr
   | .bvar j => .bvar j
   | .fvar y => if x == y then .bvar i else .fvar y
-  | .lam₁ e => .lam₁ (closing (i + 1) x e)
+  | .lam e => .lam (closing (i + 1) x e)
   | .lift e => .lift (closing i x e)
   | .app₁ f arg => .app₁ (closing i x f) (closing i x arg)
   | .app₂ f arg => .app₂ (closing i x f) (closing i x arg)
-  | .lit₁ n => .lit₁ n
+  | .lit n => .lit n
   | .binary₁ op l r => .binary₁ op (closing i x l) (closing i x r)
   | .binary₂ op l r => .binary₂ op (closing i x l) (closing i x r)
   | .run e => .run (closing i x e)
@@ -108,11 +108,11 @@ def closed_at (e : Expr) (f : ℕ) : Prop :=
   match e with
   | .bvar _ => true
   | .fvar x => x < f
-  | .lam₁ e => closed_at e f
+  | .lam e => closed_at e f
   | .lift e => closed_at e f
   | .app₁ e1 e2 => closed_at e1 f ∧ closed_at e2 f
   | .app₂ e1 e2 => closed_at e1 f ∧ closed_at e2 f
-  | .lit₁ _ => true
+  | .lit _ => true
   | .binary₁ _ l r => closed_at l f ∧ closed_at r f
   | .binary₂ _ l r => closed_at l f ∧ closed_at r f
   | .run e => closed_at e f
@@ -139,11 +139,11 @@ def closedb_at (e : Expr) (b : ℕ) : Prop :=
   match e with
   | .bvar x => x < b
   | .fvar _ => true
-  | .lam₁ e => closedb_at e (b + 1)
+  | .lam e => closedb_at e (b + 1)
   | .lift e => closedb_at e b
   | .app₁ e1 e2 => closedb_at e1 b ∧ closedb_at e2 b
   | .app₂ e1 e2 => closedb_at e1 b ∧ closedb_at e2 b
-  | .lit₁ _ => true
+  | .lit _ => true
   | .binary₁ _ l r => closedb_at l b ∧ closedb_at r b
   | .binary₂ _ l r => closedb_at l b ∧ closedb_at r b
   | .run e => closedb_at e b
@@ -172,11 +172,11 @@ def maping𝕔 (e : Expr) (i : ℕ) : Expr :=
   match e with
   | .bvar j => if j == i then (.code (.bvar i)) else .bvar j
   | .fvar x => .fvar x
-  | .lam₁ e => .lam₁ (maping𝕔 e (i + 1))
+  | .lam e => .lam (maping𝕔 e (i + 1))
   | .lift e => .lift (maping𝕔 e i)
   | .app₁ f arg => .app₁ (maping𝕔 f i) (maping𝕔 arg i)
   | .app₂ f arg => .app₂ (maping𝕔 f i) (maping𝕔 arg i)
-  | .lit₁ n => .lit₁ n
+  | .lit n => .lit n
   | .binary₁ op l r => .binary₁ op (maping𝕔 l i) (maping𝕔 r i)
   | .binary₂ op l r => .binary₂ op (maping𝕔 l i) (maping𝕔 r i)
   | .run e => .run (maping𝕔 e i)
@@ -204,11 +204,11 @@ def map𝕔₀ (e : Expr) : Expr := maping𝕔 e 0
 def fv : Expr → Set ℕ
   | .bvar _ => ∅
   | .fvar x => { x }
-  | .lam₁ e => fv e
+  | .lam e => fv e
   | .lift e => fv e
   | .app₁ f arg => fv f ∪ fv arg
   | .app₂ f arg => fv f ∪ fv arg
-  | .lit₁ _ => ∅
+  | .lit _ => ∅
   | .binary₁ _ l r => fv l ∪ fv r
   | .binary₂ _ l r => fv l ∪ fv r
   | .run e => fv e
@@ -240,7 +240,7 @@ lemma subst_intro : ∀ x e v i, closed_at e x → subst x v (opening i (.fvar x
     . simp [if_neg HEq]
   | fvar y =>
     simp at *; omega
-  | lam₁ _ IH
+  | lam _ IH
   | lift _ IH
   | code _ IH
   | reflect _ IH
@@ -264,7 +264,7 @@ lemma subst_intro : ∀ x e v i, closed_at e x → subst x v (opening i (.fvar x
     simp; constructor
     apply IH₀; apply Hclosed.left
     apply IH₁; apply Hclosed.right
-  | lit₁| loc => simp
+  | lit| loc => simp
   | ifz₁ _ _ _ IH₀ IH₁ IH₂
   | ifz₂ _ _ _ IH₀ IH₁ IH₂ =>
     simp; constructor
@@ -278,7 +278,7 @@ lemma subst_closed_id : ∀ x e v, closed_at e x → subst x v e = e :=
   induction e with
   | bvar => simp
   | fvar => simp at *; omega
-  | lam₁ _ IH
+  | lam _ IH
   | lift _ IH
   | lam𝕔 _ IH
   | code _ IH
@@ -305,7 +305,7 @@ lemma subst_closed_id : ∀ x e v, closed_at e x → subst x v e = e :=
     simp; constructor
     apply IHb; apply He.left
     apply IH; apply He.right
-  | lit₁| loc => simp
+  | lit| loc => simp
   | ifz₁ _ _ _ IH₀ IH₁ IH₂
   | ifz₂ _ _ _ IH₀ IH₁ IH₂ =>
     simp; constructor
@@ -326,7 +326,7 @@ lemma closedb_inc: ∀ t i j,
   induction t generalizing i j with
   | bvar => simp at *; omega
   | fvar => simp
-  | lam₁ _ IH
+  | lam _ IH
   | lift _ IH
   | lam𝕔 _ IH
   | code _ IH
@@ -350,7 +350,7 @@ lemma closedb_inc: ∀ t i j,
     apply And.intro
     . apply IH₀; apply Hclose.left; omega
     . apply IH₁; apply Hclose.right; omega
-  | lit₁| loc => simp
+  | lit| loc => simp
   | ifz₁ _ _ _ IH₀ IH₁ IH₂
   | ifz₂ _ _ _ IH₀ IH₁ IH₂ =>
     simp; constructor
@@ -375,8 +375,8 @@ lemma closed_inc : ∀ x y e, closed_at e x → x ≤ y → closed_at e y :=
     simp; constructor
     apply IH₀; apply Hclose.left
     apply IH₁; apply Hclose.right
-  | lit₁| loc => simp
-  | lam₁ _ IH
+  | lit| loc => simp
+  | lam _ IH
   | lift _ IH
   | lam𝕔 _ IH
   | code _ IH
@@ -405,7 +405,7 @@ lemma subst_closedb_at : ∀ x e v i, closedb_at v i → closedb_at e i → clos
     by_cases HEq : x = y
     . rw [HEq]; simp; apply Hv
     . simp; rw [if_neg HEq]; simp
-  | lam₁ _ IH
+  | lam _ IH
   | lift _ IH
   | lam𝕔 _ IH =>
     apply IH; apply closedb_inc; apply Hv; omega; apply He
@@ -433,7 +433,7 @@ lemma subst_closedb_at : ∀ x e v i, closedb_at v i → closedb_at e i → clos
   | fix₁ _ IH
   | fix₂ _ IH =>
     simp; apply IH; apply Hv; apply He
-  | lit₁| loc => simp
+  | lit| loc => simp
   | ifz₁ _ _ _ IH₀ IH₁ IH₂
   | ifz₂ _ _ _ IH₀ IH₁ IH₂ =>
     simp; constructor
@@ -450,7 +450,7 @@ lemma subst_closed_at : ∀ x e v y, closed_at v y → closed_at e y → closed_
     by_cases HEq : x = z
     . rw [HEq]; simp; apply Hv
     . simp; rw [if_neg HEq]; apply He
-  | lam₁ _ IH
+  | lam _ IH
   | lift _ IH
   | lam𝕔 _ IH =>
     apply IH; apply Hv; apply He
@@ -475,7 +475,7 @@ lemma subst_closed_at : ∀ x e v y, closed_at v y → closed_at e y → closed_
   | fix₁ _ IH
   | fix₂ _ IH =>
     simp; apply IH; apply Hv; apply He
-  | lit₁| loc => simp
+  | lit| loc => simp
   | ifz₁ _ _ _ IH₀ IH₁ IH₂
   | ifz₂ _ _ _ IH₀ IH₁ IH₂ =>
     simp; constructor
@@ -492,7 +492,7 @@ lemma subst_closed_at_dec : ∀ x e v, closed_at v x → closed_at e (x + 1) →
     by_cases HEq : x = z
     . rw [← HEq]; simp; apply Hv
     . simp; rw [if_neg HEq]; simp at *; omega
-  | lam₁ _ IH
+  | lam _ IH
   | lift _ IH
   | lam𝕔 _ IH =>
     apply IH; apply He
@@ -517,7 +517,7 @@ lemma subst_closed_at_dec : ∀ x e v, closed_at v x → closed_at e (x + 1) →
   | fix₁ _ IH
   | fix₂ _ IH =>
     simp; apply IH; apply He
-  | lit₁| loc => simp
+  | lit| loc => simp
   | ifz₁ _ _ _ IH₀ IH₁ IH₂
   | ifz₂ _ _ _ IH₀ IH₁ IH₂ =>
     simp; constructor
@@ -536,8 +536,8 @@ lemma open_closedb : ∀ i x e, closedb_at (opening i (.fvar x) e) i ↔ closedb
       . simp
     . rw [if_neg HEq]; simp; omega
   | fvar => simp
-  | lit₁| loc => simp
-  | lam₁ _ IH
+  | lit| loc => simp
+  | lam _ IH
   | lift _ IH
   | lam𝕔 _ IH
   | code _ IH
@@ -590,7 +590,7 @@ lemma close_closed : ∀ e x i, closed_at e (x + 1) ↔ closed_at (closing i x e
     . rw [HEq]; simp
     . simp; rw [if_neg HEq]; simp; omega
   | bvar => simp
-  | lam₁ _ IH
+  | lam _ IH
   | lift _ IH
   | lam𝕔 _ IH
   | code _ IH
@@ -618,7 +618,7 @@ lemma close_closed : ∀ e x i, closed_at e (x + 1) ↔ closed_at (closing i x e
     . intro Hclose; constructor
       apply (IH₀ _).mpr; apply Hclose.left
       apply (IH₁ _).mpr; apply Hclose.right
-  | lit₁| loc => simp
+  | lit| loc => simp
   | ifz₁ _ _ _ IH₀ IH₁ IH₂
   | ifz₂ _ _ _ IH₀ IH₁ IH₂ =>
     constructor
@@ -642,8 +642,8 @@ lemma open_subst_closed : ∀ x e v i, closed_at e x → closed_at v x → close
     . rw [if_pos HEq]; apply Hv
     . rw [if_neg HEq]; simp
   | fvar => apply He
-  | lit₁| loc => simp
-  | lam₁ _ IH
+  | lit| loc => simp
+  | lam _ IH
   | lift _ IH
   | lam𝕔 _ IH
   | code _ IH
@@ -683,7 +683,7 @@ lemma open_closed : ∀ e x i, closed_at e x → closed_at (opening i (.fvar x) 
     by_cases HEq : j = i
     . rw [HEq]; simp
     . simp; rw [if_neg HEq]; simp
-  | lam₁ _ IH
+  | lam _ IH
   | lift _ IH
   | lam𝕔 _ IH
   | code _ IH
@@ -707,7 +707,7 @@ lemma open_closed : ∀ e x i, closed_at e x → closed_at (opening i (.fvar x) 
     intro Hclose; constructor
     apply IH₀; apply Hclose.left
     apply IH₁; apply Hclose.right
-  | lit₁| loc => simp
+  | lit| loc => simp
   | ifz₁ _ _ _ IH₀ IH₁ IH₂
   | ifz₂ _ _ _ IH₀ IH₁ IH₂ =>
     intro Hclose; constructor
@@ -724,7 +724,7 @@ lemma close_closedb : ∀ e x i j, j < i → closedb_at e i → closedb_at (clos
     . rw [HEq]; simp; omega
     . simp; rw [if_neg HEq]; simp
   | bvar => simp
-  | lam₁ _ IH
+  | lam _ IH
   | lift _ IH
   | lam𝕔 _ IH
   | code _ IH
@@ -748,7 +748,7 @@ lemma close_closedb : ∀ e x i j, j < i → closedb_at e i → closedb_at (clos
     intro Hclose; constructor
     apply IH₀; omega; apply Hclose.left
     apply IH₁; omega; apply Hclose.right
-  | lit₁| loc => simp
+  | lit| loc => simp
   | ifz₁ _ _ _ IH₀ IH₁ IH₂
   | ifz₂ _ _ _ IH₀ IH₁ IH₂ =>
     intro Hclose; constructor
@@ -766,7 +766,7 @@ lemma closedb_opening_id : ∀ e v i, closedb_at e i → opening i v e = e :=
   | code _ IH
   | reflect _ IH
   | run _ IH
-  | lam₁ _ IH
+  | lam _ IH
   | lam𝕔 _ IH
   | load₁ _ IH
   | alloc₁ _ IH
@@ -786,7 +786,7 @@ lemma closedb_opening_id : ∀ e v i, closedb_at e i → opening i v e = e :=
     simp; constructor
     apply IH₀; apply Hclosedb.left
     apply IH₁; apply Hclosedb.right
-  | lit₁| loc => simp
+  | lit| loc => simp
   | ifz₁ _ _ _ IH₀ IH₁ IH₂
   | ifz₂ _ _ _ IH₀ IH₁ IH₂ =>
     simp; constructor
@@ -808,7 +808,7 @@ lemma open_close_id : ∀ i e x, closedb_at e i → opening i (.fvar x) (closing
     by_cases HEq : x = y
     . rw [HEq]; simp
     . rw [if_neg HEq]; simp
-  | lam₁ _ IH
+  | lam _ IH
   | lift _ IH
   | lam𝕔 _ IH
   | code _ IH
@@ -832,7 +832,7 @@ lemma open_close_id : ∀ i e x, closedb_at e i → opening i (.fvar x) (closing
     simp; constructor
     apply IH₀; apply Hlc.left
     apply IH₁; apply Hlc.right
-  | lit₁| loc => rfl
+  | lit| loc => rfl
   | ifz₁ _ _ _ IH₀ IH₁ IH₂
   | ifz₂ _ _ _ IH₀ IH₁ IH₂ =>
     simp; constructor
@@ -851,7 +851,7 @@ lemma close_open_id : ∀ i e x, closed_at e x → closing i x (opening i (.fvar
     . simp; rw [if_pos HEq]; simp; omega
     . simp; rw [if_neg HEq]; simp
   | fvar y => simp at *; omega
-  | lam₁ _ IH
+  | lam _ IH
   | lift _ IH
   | lam𝕔 _ IH
   | code _ IH
@@ -875,7 +875,7 @@ lemma close_open_id : ∀ i e x, closed_at e x → closing i x (opening i (.fvar
     simp; constructor
     apply IH₀; apply Hclose.left
     apply IH₁; apply Hclose.right
-  | lit₁| loc => rfl
+  | lit| loc => rfl
   | ifz₁ _ _ _ IH₀ IH₁ IH₂
   | ifz₂ _ _ _ IH₀ IH₁ IH₂ =>
     simp; constructor
@@ -922,8 +922,8 @@ lemma subst_opening_comm :
   | fix₁ _ IH
   | fix₂ _ IH =>
     simp; apply IH; apply Hclosedb
-  | lit₁| loc => simp
-  | lam₁ _ IH
+  | lit| loc => simp
+  | lam _ IH
   | lift _ IH
   | lam𝕔 _ IH =>
     simp; apply IH; apply closedb_inc; apply Hclosedb; omega
@@ -937,7 +937,7 @@ lemma subst_opening_comm :
 lemma subst_open₀_comm : ∀ x y e v, x ≠ y → lc v → subst x v (open₀ y e) = open₀ y (subst x v e) := by
   intros x y e v; apply subst_opening_comm
 
-example : map𝕔₀ (.app₁ (.bvar 0) (.lam₁ (.bvar 1))) = .app₁ (.code (.bvar 0)) (.lam₁ (.code (.bvar 1))) := by simp
+example : map𝕔₀ (.app₁ (.bvar 0) (.lam (.bvar 1))) = .app₁ (.code (.bvar 0)) (.lam (.code (.bvar 1))) := by simp
 
 lemma maping𝕔_intro :
     ∀ x e i, closed_at e x → closing i x (subst x (.code (.fvar x)) (opening i (.fvar x) e)) = maping𝕔 e i :=
@@ -946,7 +946,7 @@ lemma maping𝕔_intro :
   induction e generalizing i with
   | bvar j => by_cases HEq : j = i; rw [HEq]; simp; simp [if_neg HEq]
   | fvar y => simp at *; by_cases HEq : x = y; omega; rw [if_neg HEq]; simp; apply HEq
-  | lam₁ _ IH
+  | lam _ IH
   | lift _ IH
   | code _ IH
   | reflect _ IH
@@ -970,7 +970,7 @@ lemma maping𝕔_intro :
     simp at *; constructor
     apply IH₀; apply Hclose.left
     apply IH₁; apply Hclose.right
-  | lit₁| loc => simp
+  | lit| loc => simp
   | ifz₁ _ _ _ IH₀ IH₁ IH₂
   | ifz₂ _ _ _ IH₀ IH₁ IH₂ =>
     simp; constructor
@@ -993,8 +993,8 @@ lemma maping𝕔_closed : ∀ x e i, closed_at e x → closed_at (maping𝕔 e i
     . rw [if_pos HEq]; apply He
     . rw [if_neg HEq]; simp
   | fvar => apply He
-  | lit₁| loc => simp
-  | lam₁ _ IH
+  | lit| loc => simp
+  | lam _ IH
   | lift _ IH
   | lam𝕔 _ IH
   | code _ IH
@@ -1037,8 +1037,8 @@ lemma fv_if_closed_at :
   | fvar z =>
     simp at *
     omega
-  | lit₁| loc => nomatch HIn
-  | lam₁ _ IH
+  | lit| loc => nomatch HIn
+  | lam _ IH
   | lift _ IH
   | lam𝕔 _ IH
   | code _ IH
@@ -1085,8 +1085,8 @@ lemma fv_opening : ∀ i v e, fv (opening i v e) ⊆ fv v ∪ fv e :=
     . rw [if_pos HEq]
     . rw [if_neg HEq]; simp
   | fvar z => simp
-  | lit₁| loc => simp
-  | lam₁ _ IH
+  | lit| loc => simp
+  | lam _ IH
   | lift _ IH
   | lam𝕔 _ IH
   | code _ IH
@@ -1149,12 +1149,12 @@ lemma fv_closed_at_dec :
   induction e with
   | bvar j => simp
   | fvar y => simp at *; omega
-  | lit₁| loc => simp
+  | lit| loc => simp
   | lift _ IH
   | code _ IH
   | reflect _ IH
   | run _ IH
-  | lam₁ _ IH
+  | lam _ IH
   | lam𝕔 _ IH
   | load₁ _ IH
   | alloc₁ _ IH
@@ -1190,8 +1190,8 @@ lemma fv_maping𝕔 : ∀ e i, fv e = fv (maping𝕔 e i) :=
     . rw [if_pos HEq]; rfl
     . rw [if_neg HEq]; rfl
   | fvar => rfl
-  | lit₁| loc => rfl
-  | lam₁ _ IH
+  | lit| loc => rfl
+  | lam _ IH
   | lift _ IH
   | lam𝕔 _ IH
   | code _ IH
@@ -1222,8 +1222,8 @@ lemma fv_empty_iff_closed : ∀ e, fv e = ∅ ↔ closed_at e 0 :=
   induction e with
   | bvar => simp
   | fvar => simp
-  | lit₁| loc => simp
-  | lam₁ _ IH
+  | lit| loc => simp
+  | lam _ IH
   | lift _ IH
   | lam𝕔 _ IH
   | code _ IH
@@ -1279,8 +1279,8 @@ lemma fv_closing : ∀ i x e, fv (closing i x e) = fv e \ { x } :=
     . rw [if_neg HEq]
       rw [Set.diff_singleton_eq_self]
       rfl; apply HEq
-  | lit₁| loc => simp
-  | lam₁ _ IH
+  | lit| loc => simp
+  | lam _ IH
   | lift _ IH
   | lam𝕔 _ IH
   | code _ IH
@@ -1317,7 +1317,7 @@ lemma fv_subset_closed :
   by
   intros e₀ e₁ x HFv Hclose
   induction e₁ with
-  | bvar| lit₁| loc => simp
+  | bvar| lit| loc => simp
   | fvar y =>
     simp at *
     have _ : ¬y ≥ x := by
@@ -1325,7 +1325,7 @@ lemma fv_subset_closed :
       apply fv_if_closed_at; apply Hclose
       apply HGe; apply HFv
     omega
-  | lam₁ _ IH
+  | lam _ IH
   | lift _ IH
   | lam𝕔 _ IH
   | code _ IH
