CollapsingTowers/TwoLevelPCP/Shift.lean
@@ -6,11 +6,11 @@ import CollapsingTowers.TwoLevelPCP.OpenClose
 def shiftl_at (x : ℕ) (n : ℕ) : Expr → Expr
   | .bvar i => .bvar i
   | .fvar y => if x ≤ y then .fvar (y + n) else .fvar y
-  | .lam₁ e => .lam₁ (shiftl_at x n e)
+  | .lam e => .lam (shiftl_at x n e)
   | .lift e => .lift (shiftl_at x n e)
   | .app₁ f arg => .app₁ (shiftl_at x n f) (shiftl_at x n arg)
   | .app₂ f arg => .app₂ (shiftl_at x n f) (shiftl_at x n arg)
-  | .lit₁ n => .lit₁ n
+  | .lit n => .lit n
   | .binary₁ op l r => .binary₁ op (shiftl_at x n l) (shiftl_at x n r)
   | .binary₂ op l r => .binary₂ op (shiftl_at x n l) (shiftl_at x n r)
   | .run e => .run (shiftl_at x n e)
@@ -35,11 +35,11 @@ def shiftl_at (x : ℕ) (n : ℕ) : Expr → Expr
 def shiftr_at (x : ℕ) : Expr → Expr
   | .bvar i => .bvar i
   | .fvar y => if x < y then .fvar (y - 1) else .fvar y
-  | .lam₁ e => .lam₁ (shiftr_at x e)
+  | .lam e => .lam (shiftr_at x e)
   | .lift e => .lift (shiftr_at x e)
   | .app₁ f arg => .app₁ (shiftr_at x f) (shiftr_at x arg)
   | .app₂ f arg => .app₂ (shiftr_at x f) (shiftr_at x arg)
-  | .lit₁ n => .lit₁ n
+  | .lit n => .lit n
   | .binary₁ op l r => .binary₁ op (shiftr_at x l) (shiftr_at x r)
   | .binary₂ op l r => .binary₂ op (shiftr_at x l) (shiftr_at x r)
   | .run e => .run (shiftr_at x e)
@@ -82,8 +82,8 @@ theorem shiftl_opening_comm :
   | store₁ _ _ IH₀ IH₁
   | store₂ _ _ IH₀ IH₁ =>
     simp; constructor; apply IH₀; apply IH₁
-  | lit₁| loc => simp
-  | lam₁ _ IH
+  | lit| loc => simp
+  | lam _ IH
   | lift _ IH
   | lam𝕔 _ IH
   | code _ IH
@@ -126,8 +126,8 @@ theorem shiftl_closed_at :
     simp; constructor
     apply IH₀; apply Hclose.left
     apply IH₁; apply Hclose.right
-  | lit₁| loc => simp
-  | lam₁ _ IH
+  | lit| loc => simp
+  | lam _ IH
   | lift _ IH
   | lam𝕔 _ IH
   | code _ IH
@@ -165,8 +165,8 @@ theorem shiftl_id :
     intro Hclose; simp; constructor
     apply IH₀; apply Hclose.left
     apply IH₁; apply Hclose.right
-  | lit₁| loc => simp
-  | lam₁ _ IH
+  | lit| loc => simp
+  | lam _ IH
   | lift _ IH
   | lam𝕔 _ IH
   | code _ IH
@@ -208,8 +208,8 @@ theorem shiftr_opening_comm :
   | store₁ _ _ IH₀ IH₁
   | store₂ _ _ IH₀ IH₁ =>
     simp; constructor; apply IH₀; apply IH₁
-  | lit₁| loc => simp
-  | lam₁ _ IH
+  | lit| loc => simp
+  | lam _ IH
   | lift _ IH
   | lam𝕔 _ IH
   | code _ IH
@@ -253,8 +253,8 @@ theorem shiftr_closed_at : ∀ x y e, y < x → closed_at e (x + 1) → closed_a
     simp; constructor
     apply IH₀; apply Hclose.left
     apply IH₁; apply Hclose.right
-  | lit₁| loc => simp
-  | lam₁ _ IH
+  | lit| loc => simp
+  | lam _ IH
   | lift _ IH
   | lam𝕔 _ IH
   | code _ IH
@@ -294,8 +294,8 @@ theorem shiftr_closed_at_id : ∀ x e, closed_at e x → closed_at (shiftr_at x 
     simp; constructor
     apply IH₀; apply Hclose.left
     apply IH₁; apply Hclose.right
-  | lit₁| loc => simp
-  | lam₁ _ IH
+  | lit| loc => simp
+  | lam _ IH
   | lift _ IH
   | lam𝕔 _ IH
   | code _ IH
@@ -333,8 +333,8 @@ theorem shiftr_id :
     intro Hclose; simp; constructor
     apply IH₀; apply Hclose.left
     apply IH₁; apply Hclose.right
-  | lit₁| loc => simp
-  | lam₁ _ IH
+  | lit| loc => simp
+  | lam _ IH
   | lift _ IH
   | lam𝕔 _ IH
   | code _ IH
